proofs/x86-64/avx2/ml_dsa_65/row_vector.ec
@@ -216,20 +216,90 @@ lemma row_vector____multiply_with_matrix_A_correct
       (_mat : W32.t Array7680.t) (_vec : W32.t Array1280.t) :
     hoare [ M.row_vector____multiply_with_matrix_A :
         matrix_A = _mat /\ vector = _vec /\
+        wpolymat_urng (mat_unflatten256 _mat) q /\
         wpolylvec_bmul_irng (lvec_unflatten256 _vec)
-        (* matrix_A range: each row is a polylvec with bmul_irng *)
         ==>
         lifts_wpolykvec (kvec_unflatten256 res) =
           ntt_mulmxv (liftu_wpolymat (mat_unflatten256 _mat))
                      (lifts_wpolylvec (lvec_unflatten256 _vec))
     ].
 proof.
-admitted.
+have lvec_val := mldsa65_lvec.
+have kvec_val := mldsa65_kvec.
+proc.
+while (0 <= i <= 6 /\ matrix_A = _mat /\ vector = _vec /\
+       wpolymat_urng (mat_unflatten256 _mat) q /\
+       wpolylvec_bmul_irng (lvec_unflatten256 _vec) /\
+       (forall k, 0 <= k < i =>
+          (lifts_wpolykvec (kvec_unflatten256 out)).[k] =
+          ntt_dotp (row (lifts_wpolymat (mat_unflatten256 _mat)) k)
+                   (lifts_wpolylvec (lvec_unflatten256 _vec)))); last first.
++ (* Exit + pre-loop *)
+  auto => /> Hmurng Hvbmul; split; 1: smt().
+  move => i out Hng Hi1 Hi2 Hinv; have {Hi2} Hi2 : i = 6 by smt().
+  subst i.
+  (* lifts_wpolymat = liftu_wpolymat under urng q *)
+  have Hlifts_eq_liftu :
+      lifts_wpolymat (mat_unflatten256 _mat) = liftu_wpolymat (mat_unflatten256 _mat).
+  + rewrite /lifts_wpolymat /liftu_wpolymat.
+    apply KLMatrix.tP => j jb.
+    rewrite !mapiE 1,2:/# /=.
+    move: Hmurng; rewrite /wpolymat_urng KLMatrix.allP => Hj.
+    apply wpoly_urng_lifts_eq_liftu.
+    by apply (Hj j _); smt().
+  rewrite /ntt_mulmxv; apply KArray.tP => k kb.
+  rewrite KArray.initiE 1:/# /= -Hlifts_eq_liftu.
+  by apply (Hinv k _); smt().
+
+(* Loop body *)
+wp; ecall (row_vector____dot_product_correct
+            (Array256.init (fun j => out.[256 * i + j]))
+            (Array1280.init (fun j => matrix_A.[5 * 256 * i + j]))
+            vector).
+auto => /> &hr Hi1 Hi2 Hmurng Hvbmul Hinv Hguard.
+split.
++ (* wpolylvec_bmul_irng on row slice: each element is urng q and hence bmul_irng *)
+  rewrite /wpolylvec_bmul_irng LArray.allP => l lb.
+  have /= -> := mat_row_slice_unflatten _mat i{hr} l _ _; 1,2: smt().
+  apply wpoly_urng_bmul_irng.
+  move: Hmurng; rewrite /wpolymat_urng KLMatrix.allP => Hj.
+  by apply (Hj (i{hr}*lvec + l) _); smt().
++ (* Post-call: establish invariant at i+1 *)
+  move => _ aux Haux.
+  do split; 1,2: smt().
+  move => k kl ku.
+  have /= Hwb :=
+    kvec_unflatten256_writeback_iE out{hr} aux (256 * i{hr}) k _ _; 1,2: smt().
+  rewrite /lifts_wpolykvec mapiE; 1: smt(mldsa65_kvec).
+  rewrite Hwb.
+  case (k = i{hr}) => Hki.
+  + (* New row: k = i *)
+    subst k.
+    have -> : 256 * i{hr} %/ 256 = i{hr} by smt().
+    rewrite ifT // Haux.
+    (* Row slice of matrix = row of lifts_wpolymat *)
+    have -> : (Array1280.init (fun j => _mat.[5 * 256 * i{hr} + j])) =
+              (Array1280.init (fun j => _mat.[1280 * i{hr} + j])).
+    + by apply Array1280.tP => j jb; rewrite !Array1280.initiE 1,2:/# /= /#.
+    congr.
+    (* lifts_wpolylvec (lvec_unflatten256 row_slice) = row (lifts_wpolymat _) i *)
+    apply LArray.tP => l lb.
+    rewrite /lifts_wpolylvec mapiE 1:/# /=.
+    have /= -> := mat_row_slice_unflatten _mat i{hr} l _ _; 1,2: smt().
+    rewrite /row LArray.initiE 1:/# /=.
+    by rewrite /lifts_wpolymat mapiE 1:/#.
+  + (* Old row: k < i *)
+    have -> : (k = 256 * i{hr} %/ 256) = false by smt().
+    rewrite /=.
+    have /= := Hinv k _; 1: smt().
+    by rewrite /lifts_wpolykvec mapiE 1:/#.
+qed.
 
 lemma row_vector____multiply_with_matrix_A_ph
       (_mat : W32.t Array7680.t) (_vec : W32.t Array1280.t) :
     phoare [ M.row_vector____multiply_with_matrix_A :
         matrix_A = _mat /\ vector = _vec /\
+        wpolymat_urng (mat_unflatten256 _mat) q /\
         wpolylvec_bmul_irng (lvec_unflatten256 _vec)
         ==>
         lifts_wpolykvec (kvec_unflatten256 res) =
